lib/List.dfy
@@ -1,0 +1,10 @@
+module ListModule {
+
+  datatype List<T> = Nil | Cons(head: T, tail: List<T>)
+
+  function ToSeq<T>(xs: List<T>): seq<T> {
+    if xs.Nil? then [] else [xs.head] + ToSeq(xs.tail)
+  }
+
+}
+
